Associate keys with names rather than just predicates.

crypto1.v
@@ -113,6 +113,30 @@ Canonical levelO := leibnizO level.
 
 Implicit Types lvl : level.
 
+Global Instance level_eq_dec : EqDecision level.
+Proof.
+refine (λ lvl1 lvl2,
+          match lvl1, lvl2 with
+          | Pub, Pub | Sec, Sec => left eq_refl
+          | _, _ => right _
+          end); abstract intuition congruence.
+Defined.
+
+Definition bool_of_level lvl :=
+  if lvl is Pub then false else true.
+
+Definition level_of_bool (b : bool) :=
+  if b then Sec else Pub.
+
+Lemma bool_of_levelK : Cancel (=) level_of_bool bool_of_level.
+Proof. by case. Qed.
+
+Global Instance level_countable : Countable level.
+Proof.
+eapply @inj_countable'; last by eapply bool_of_levelK.
+apply _.
+Qed.
+
 Global Instance level_sqsubseteq : SqSubsetEq level := λ lvl1 lvl2,
   match lvl1, lvl2 with
   | Sec, Pub => False
@@ -164,99 +188,76 @@ Implicit Types γ : gname.
 
 Inductive res :=
 | RNonce of level
-| RAKey of level & level & termO -n> iPropO Σ
-| RSKey of level & termO -n> iPropO Σ.
+| RAKey of level & level & gname (* was: Predicate *)
+| RSKey of level & gname.
 
-Global Instance res_equiv : Equiv res := λ r1 r2,
-  match r1, r2 with
-  | RNonce lvl1, RNonce lvl2 => lvl1 = lvl2
-  | RAKey lvl11 lvl12 P1, RAKey lvl21 lvl22 P2 =>
-    lvl11 = lvl21 ∧ lvl12 = lvl22 ∧ P1 ≡ P2
-  | RSKey lvl1 P1, RSKey lvl2 P2 => lvl1 = lvl2 ∧ P1 ≡ P2
-  | _, _ => False
+Canonical resO := leibnizO res.
+
+Implicit Types r : res.
+
+Definition sum_of_res r :=
+  match r with
+  | RNonce lvl => inl lvl
+  | RAKey lvl_enc lvl_dec γ => inr (inl (lvl_enc, lvl_dec, γ))
+  | RSKey lvl γ => inr (inr (lvl, γ))
   end.
 
-Global Instance res_dist : Dist res := λ n r1 r2,
-  match r1, r2 with
-  | RNonce lvl1, RNonce lvl2 => lvl1 = lvl2
-  | RAKey lvl11 lvl12 P1, RAKey lvl21 lvl22 P2 =>
-    lvl11 = lvl21 ∧ lvl12 = lvl22 ∧ P1 ≡{n}≡ P2
-  | RSKey lvl1 P1, RSKey lvl2 P2 => lvl1 = lvl2 ∧ P1 ≡{n}≡ P2
-  | _, _ => False
+Definition res_of_sum x :=
+  match x with
+  | inl lvl => RNonce lvl
+  | inr (inl (lvl_enc, lvl_dec, γ)) => RAKey lvl_enc lvl_dec γ
+  | inr (inr (lvl, γ)) => RSKey lvl γ
   end.
 
-Lemma res_ofe_mixin : OfeMixin res.
-Proof.
-split.
-- move=> r1 r2; case: r1=> *; case: r2=> *;
-  rewrite /equiv /dist /= ?forall_and_distr ?equiv_dist;
-  intuition eauto using 0.
-- rewrite /dist; move=> n; split.
-  + case=> * //=; by apply equiv_dist.
-  + case=> [lvl1|lvl11 lvl12 P1|lvl1 P1] [lvl2|lvl21 lvl22 P2|lvl2 P2] //=;
-    intuition eauto.
-  + case=> [?|???|??] [?|???|??] //= [?|???|??] //=;
-    intuition (try congruence); etransitivity; eauto.
-- rewrite /dist => n [?|???|??] [?|???|??] //=;
-  intuition eauto using dist_S.
-Qed.
-Canonical resO := OfeT res res_ofe_mixin.
-
-Lemma res_equivI (r1 r2 : res) :
-  r1 ≡ r2 ⊣⊢@{iPropI Σ}
-  match r1, r2 with
-  | RNonce lvl1, RNonce lvl2 => ⌜lvl1 = lvl2⌝
-  | RAKey lvl_enc1 lvl_dec1 Φ1, RAKey lvl_enc2 lvl_dec2 Φ2 =>
-    ⌜lvl_enc1 = lvl_enc2⌝ ∧ ⌜lvl_dec1 = lvl_dec2⌝ ∧ Φ1 ≡ Φ2
-  | RSKey lvl1 Φ1, RSKey lvl2 Φ2 =>
-    ⌜lvl1 = lvl2⌝ ∧ Φ1 ≡ Φ2
-  | _, _ => False
-  end.
-Proof. case: r1=> *; case: r2=> * /=; by uPred.unseal. Qed.
-
-Global Instance discrete_RNonce lvl : Discrete (RNonce lvl).
+Lemma sum_of_resK : Cancel (=) res_of_sum sum_of_res.
 Proof. by case. Qed.
 
+Global Instance res_eq_dec : EqDecision res.
+Proof.
+refine (λ r1 r2,
+         match r1, r2 with
+         | RNonce lvl1, RNonce lvl2 =>
+           cast_if (decide (lvl1 = lvl2))
+         | RAKey lvl_enc1 lvl_dec1 γ1, RAKey lvl_enc2 lvl_dec2 γ2 =>
+           cast_if_and3 (decide (lvl_enc1 = lvl_enc2))
+                        (decide (lvl_dec1 = lvl_dec2))
+                        (decide (γ1 = γ2))
+         | RSKey lvl1 γ1, RSKey lvl2 γ2 =>
+           cast_if_and (decide (lvl1 = lvl2)) (decide (γ1 = γ2))
+         | _, _ => right _
+         end); abstract intuition congruence.
+Defined.
+
+Global Instance res_countable : Countable res.
+Proof.
+eapply (inj_countable' _ _ sum_of_resK).
+Qed.
+
 Class resG := {
-  res_inG :> inG Σ (agreeR resO);
+  res_inG :> inG Σ (optionUR (agreeR (termO -n> iPropO Σ)));
 }.
 
 Context `{!resG, !heapG Σ}.
 
 Definition resT r l : iProp Σ :=
-  ∃ γ, meta l (cryptoN.@"res") γ ∗ own γ (to_agree r).
+  meta l (cryptoN.@"res") r.
 
 Lemma resT_persistent r l : Persistent (resT r l).
 Proof. apply _. Qed.
 
-Lemma resT_agree r1 r2 l : resT r1 l -∗ resT r2 l -∗ r1 ≡ r2.
-Proof.
-iDestruct 1 as (γ) "[#Hl #Hγ]".
-iDestruct 1 as (γ') "[#Hl' #Hγ']".
-iPoseProof (meta_agree with "Hl Hl'") as "<-".
-iPoseProof (own_valid_2 with "Hγ Hγ'") as "Hvalid".
-by rewrite agree_validI agree_equivI.
-Qed.
+Lemma resT_agree r1 r2 l : resT r1 l -∗ resT r2 l -∗ ⌜r1 = r2⌝.
+Proof. exact: meta_agree. Qed.
 
-Lemma later_resT r l :
-  ▷ resT r l -∗ ◇ ∃ r', resT r' l ∗ ▷ (r ≡ r').
-Proof.
-iDestruct 1 as (γ) "[> #Hmeta Hown]".
-iMod (later_own with "Hown") as (ag) "[#Hown #Hr]".
-iPoseProof (own_valid with "Hown") as "#Hvalid".
-iDestruct (to_agree_uninjI with "Hvalid") as (r') "Hr'".
-iRewrite -"Hr'" in "Hr"; iRewrite -"Hr'" in "Hown"; rewrite agree_equivI.
-iModIntro; iExists r'; iSplit=> //.
-by iExists γ; iSplit.
-Qed.
+Lemma resT_timeless r l : Timeless (resT r l).
+Proof. apply _. Qed.
 
 Definition nonceT lvl l : iProp Σ := resT (RNonce lvl) l.
 
 Lemma nonceT_agree lvl1 lvl2 l : nonceT lvl1 l -∗ nonceT lvl2 l -∗ ⌜lvl1 = lvl2⌝.
 Proof.
 iIntros "Hown1 Hown2".
-iPoseProof (resT_agree with "Hown1 Hown2") as "#Hvalid".
-by rewrite res_equivI.
+iPoseProof (resT_agree with "Hown1 Hown2") as "%Hvalid".
+by case: Hvalid.
 Qed.
 
 Global Instance persistent_nonceT lvl l : Persistent (nonceT lvl l).
@@ -265,74 +266,104 @@ Proof. apply _. Qed.
 Global Instance timeless_nonceT lvl l : Timeless (nonceT lvl l).
 Proof. apply _. Qed.
 
-Definition akeyT lvl_enc lvl_dec Φ l : iProp Σ :=
-  resT (RAKey lvl_enc lvl_dec Φ) l.
+Definition akeyT lvl_enc lvl_dec γ Φ l : iProp Σ :=
+  resT (RAKey lvl_enc lvl_dec γ) l ∗
+  own γ (Some (to_agree Φ)).
 
-Global Instance persistent_akeyT lvl_enc lvl_dec Φ l :
-  Persistent (akeyT lvl_enc lvl_dec Φ l).
+Global Instance persistent_akeyT lvl_enc lvl_dec γ Φ l :
+  Persistent (akeyT lvl_enc lvl_dec γ Φ l).
 Proof. apply _. Qed.
 
-Definition skeyT lvl Φ l : iProp Σ := resT (RSKey lvl Φ) l.
-
-Global Instance persistent_skeyT lvl Φ l :
-  Persistent (skeyT lvl Φ l).
-Proof. apply _. Qed.
-
-Definition keyT kt rs Φ l : iProp Σ :=
-  match kt with
-  | KSym => skeyT rs Φ l
-  | KAEnc => ∃ rs_dec, akeyT rs rs_dec Φ l
-  | KADec => ∃ rs_enc, akeyT rs_enc rs Φ l
-  end.
-
-Lemma keyT_agree kt rs1 rs2 Φ1 Φ2 l :
-  keyT kt rs1 Φ1 l -∗ keyT kt rs2 Φ2 l -∗ ⌜rs1 = rs2⌝ ∗ Φ1 ≡ Φ2.
+Lemma akeyT_agree lvl_enc1 lvl_enc2 lvl_dec1 lvl_dec2 γ1 γ2 Φ1 Φ2 l :
+  akeyT lvl_enc1 lvl_dec1 γ1 Φ1 l -∗
+  akeyT lvl_enc2 lvl_dec2 γ2 Φ2 l -∗
+  ⌜lvl_enc1 = lvl_enc2⌝ ∗
+  ⌜lvl_dec1 = lvl_dec2⌝ ∗
+  ⌜γ1 = γ2⌝ ∗
+  Φ1 ≡ Φ2.
 Proof.
-case: kt=> /=.
-- iIntros "Hown1 Hown2".
-  iPoseProof (resT_agree with "Hown1 Hown2") as "#Hvalid".
-  by rewrite res_equivI /=; iDestruct "Hvalid" as "(?&?)"; iSplit.
-- iDestruct 1 as (rs1') "Hown1".
-  iDestruct 1 as (rs2') "Hown2".
-  iPoseProof (resT_agree with "Hown1 Hown2") as "#Hvalid".
-  rewrite res_equivI.
-  by iDestruct "Hvalid" as "(?&?&?)"; iSplit.
-- iDestruct 1 as (rs1') "Hown1".
-  iDestruct 1 as (rs2') "Hown2".
-  iPoseProof (resT_agree with "Hown1 Hown2") as "#Hvalid".
-  rewrite res_equivI.
-  by iDestruct "Hvalid" as "(?&?&?)"; iSplit.
+iIntros "[Hres1 Hown1] [Hres2 Hown2]".
+iPoseProof (resT_agree with "Hres1 Hres2") as "%Hres".
+case: Hres=> <- <- <-.
+iPoseProof (own_valid_2 with "Hown1 Hown2") as "#Hvalid".
+rewrite -Some_op uPred.option_validI agree_validI agree_equivI.
+by eauto.
 Qed.
 
-Global Instance persistent_keyT kt rs Φ l : Persistent (keyT kt rs Φ l).
+Definition skeyT lvl γ Φ l : iProp Σ :=
+  resT (RSKey lvl γ) l ∗
+  own γ (Some (to_agree Φ)).
+
+Global Instance persistent_skeyT lvl γ Φ l :
+  Persistent (skeyT lvl γ Φ l).
+Proof. apply _. Qed.
+
+Lemma skeyT_agree lvl1 lvl2 γ1 γ2 Φ1 Φ2 l :
+  skeyT lvl1 γ1 Φ1 l -∗
+  skeyT lvl2 γ2 Φ2 l -∗
+  ⌜lvl1 = lvl2⌝ ∗
+  ⌜γ1 = γ2⌝ ∗
+  Φ1 ≡ Φ2.
+Proof.
+iIntros "[Hres1 Hown1] [Hres2 Hown2]".
+iPoseProof (resT_agree with "Hres1 Hres2") as "%Hres".
+case: Hres=> <- <-.
+iPoseProof (own_valid_2 with "Hown1 Hown2") as "#Hvalid".
+rewrite -Some_op uPred.option_validI agree_validI agree_equivI.
+by eauto.
+Qed.
+
+Definition keyT kt rs γ Φ l : iProp Σ :=
+  match kt with
+  | KSym => skeyT rs γ Φ l
+  | KAEnc => ∃ rs_dec, akeyT rs rs_dec γ Φ l
+  | KADec => ∃ rs_enc, akeyT rs_enc rs γ Φ l
+  end.
+
+Lemma keyT_agree kt rs1 rs2 γ1 γ2 Φ1 Φ2 l :
+  keyT kt rs1 γ1 Φ1 l -∗ keyT kt rs2 γ2 Φ2 l -∗
+  ⌜rs1 = rs2⌝ ∗ ⌜γ1 = γ2⌝ ∗ Φ1 ≡ Φ2.
+Proof.
+case: kt=> /=.
+- by iApply skeyT_agree.
+- iDestruct 1 as (rs1') "Hres1".
+  iDestruct 1 as (rs2') "Hres2".
+  by iPoseProof (akeyT_agree with "Hres1 Hres2") as "(<-&_&<-&?)";
+  eauto.
+- iDestruct 1 as (rs1') "Hres1".
+  iDestruct 1 as (rs2') "Hres2".
+  by iPoseProof (akeyT_agree with "Hres1 Hres2") as "(<-&<-&<-&?)";
+  eauto.
+Qed.
+
+Global Instance persistent_keyT kt rs γ Φ l : Persistent (keyT kt rs γ Φ l).
 Proof. by case: kt; apply _. Qed.
 
-Definition key_info (asym : bool) lvl_enc lvl_dec Φ l : iProp Σ :=
-  if asym then akeyT lvl_enc lvl_dec Φ l
-  else (⌜lvl_enc = lvl_dec⌝ ∗ skeyT lvl_enc Φ l)%I.
+Definition key_info (asym : bool) lvl_enc lvl_dec γ Φ l : iProp Σ :=
+  if asym then akeyT lvl_enc lvl_dec γ Φ l
+  else (⌜lvl_enc = lvl_dec⌝ ∗ skeyT lvl_enc γ Φ l)%I.
 
-Lemma key_info_agree asym1 asym2 lvl_enc1 lvl_dec1 lvl_enc2 lvl_dec2  Φ1 Φ2 l :
-  key_info asym1 lvl_enc1 lvl_dec1 Φ1 l -∗
-  key_info asym2 lvl_enc2 lvl_dec2 Φ2 l -∗
-  ⌜asym1 = asym2⌝ ∗ ⌜lvl_enc1 = lvl_enc2⌝ ∗ ⌜lvl_dec1 = lvl_dec2⌝ ∗ Φ1 ≡ Φ2.
+Lemma key_info_agree asym1 asym2 lvl_enc1 lvl_dec1 lvl_enc2 lvl_dec2 γ1 γ2 Φ1 Φ2 l :
+  key_info asym1 lvl_enc1 lvl_dec1 γ1 Φ1 l -∗
+  key_info asym2 lvl_enc2 lvl_dec2 γ2 Φ2 l -∗
+  ⌜asym1 = asym2⌝ ∗ ⌜lvl_enc1 = lvl_enc2⌝ ∗ ⌜lvl_dec1 = lvl_dec2⌝ ∗
+  ⌜γ1 = γ2⌝ ∗ Φ1 ≡ Φ2.
 Proof.
 case: asym1 asym2=> [] [] /=.
 - iIntros "Hown1 Hown2".
-  iPoseProof (resT_agree with "Hown1 Hown2") as "#Hvalid".
-  by rewrite res_equivI /=; iDestruct "Hvalid" as "(?&?&?)"; repeat iSplit.
-- iIntros "Hown1 [_ Hown2]".
-  iPoseProof (resT_agree with "Hown1 Hown2") as "#Hvalid".
-  by rewrite res_equivI.
-- iIntros "[_ Hown1] Hown2".
-  iPoseProof (resT_agree with "Hown1 Hown2") as "#Hvalid".
-  by rewrite res_equivI.
+  iPoseProof (akeyT_agree with "Hown1 Hown2") as "(<-&<-&<-&?)".
+  by eauto.
+- iIntros "[Hown1 _] [_ [Hown2 _]]".
+  by iPoseProof (resT_agree with "Hown1 Hown2") as "%Hvalid".
+- iIntros "[_ [Hown1 _]] [Hown2 _]".
+  by iPoseProof (resT_agree with "Hown1 Hown2") as "%Hvalid".
 - iIntros "[<- Hown1] [<- Hown2]".
-  iPoseProof (resT_agree with "Hown1 Hown2") as "#Hvalid".
-  by rewrite res_equivI /=; iDestruct "Hvalid" as "(?&?)"; repeat iSplit.
+  iPoseProof (skeyT_agree with "Hown1 Hown2") as "(<-&<-&#Hvalid)".
+  by eauto.
 Qed.
 
-Global Instance persistent_key_info asym lvl_enc lvl_dec Φ l :
-  Persistent (key_info asym lvl_enc lvl_dec Φ l).
+Global Instance persistent_key_info asym lvl_enc lvl_dec γ Φ l :
+  Persistent (key_info asym lvl_enc lvl_dec γ Φ l).
 Proof. by case: asym; apply _. Qed.
 
 (** [termT lvl t] holds when the term [t] can be declared public after
@@ -344,10 +375,10 @@ Fixpoint termT lvl t : iProp Σ :=
   | TInt _ => True
   | TPair t1 t2 => termT lvl t1 ∗ termT lvl t2
   | TNonce l  => ∃ lvl', nonceT lvl' l ∗ ⌜lvl' ⊑ lvl⌝
-  | TKey kt l => ∃ lvl' Φ, keyT kt lvl' Φ l ∗ ⌜lvl' ⊑ lvl⌝
+  | TKey kt l => ∃ lvl' γ Φ, keyT kt lvl' γ Φ l ∗ ⌜lvl' ⊑ lvl⌝
   | TEnc asym l t =>
-    ∃ lvl_enc lvl_dec Φ,
-      key_info asym lvl_enc lvl_dec Φ l
+    ∃ lvl_enc lvl_dec γ Φ,
+      key_info asym lvl_enc lvl_dec γ Φ l
       ∗ (□ Φ t ∗ termT (lvl ⊔ lvl_dec) t ∨
          ⌜lvl_enc = Pub⌝ ∗ termT Pub t)
   end.
@@ -376,10 +407,10 @@ elim: t lvl lvl'=> [n|t1 IH1 t2 IH2|l|kt l|b l t IH] lvl lvl' sub //=.
 - by iIntros "[#Ht1 #Ht2]"; rewrite IH1 // IH2 //; iSplit.
 - iDestruct 1 as (lvl0) "[#Hnonce %sub0]".
   iExists lvl0; iSplit=> //; iPureIntro; by etransitivity.
-- iDestruct 1 as (lvl0 Φ) "[#Hkey %sub0]".
-  iExists lvl0, Φ; iSplit=> //; iPureIntro; by etransitivity.
-- iDestruct 1 as (lvl_enc lvl_dec Φ) "[#Hkey #Ht]".
-  iExists lvl_enc, lvl_dec, Φ; iSplit=> //.
+- iDestruct 1 as (lvl0 γ Φ) "[#Hkey %sub0]".
+  iExists lvl0, γ, Φ; iSplit=> //; iPureIntro; by etransitivity.
+- iDestruct 1 as (lvl_enc lvl_dec γ Φ) "[#Hkey #Ht]".
+  iExists lvl_enc, lvl_dec, γ, Φ; iSplit=> //.
   iDestruct "Ht" as "[[? Ht]|Ht]"; last by iRight.
   iLeft; iSplit=> //; iApply (IH with "Ht").
   by case: lvl lvl' lvl_dec sub=> [] [] [].
@@ -417,36 +448,36 @@ elim: t lvl=> [n|t1 IH1 t2 IH2|n|kt k|b k t IH] lvl /=.
 - iDestruct 1 as (lvl') "[#Hn %Hsub]".
   iExists lvl'; iSplit; first by iExists lvl'; eauto.
   iIntros "!> /=" (lvl''); iDestruct 1 as (lvl''') "[#Hn' %Hsub']".
-  iPoseProof (resT_agree with "Hn Hn'") as "e".
-  by rewrite res_equivI; iPoseProof "e" as "->".
-- iDestruct 1 as (lvl' Φ) "[#Hk %Hsub]".
-  iExists lvl'; iSplit; first by iExists lvl', Φ; iSplit.
-  iIntros "/= !>" (lvl''); iDestruct 1 as (lvl''' Φ') "[#Hk' %Hsub']".
-  by iPoseProof (keyT_agree with "Hk Hk'") as "(<-&_)".
+  by iPoseProof (resT_agree with "Hn Hn'") as "%e"; case: e=> ->.
+- iDestruct 1 as (lvl' γ Φ) "[#Hk %Hsub]".
+  iExists lvl'; iSplit; first by iExists lvl', γ, Φ; iSplit.
+  iIntros "/= !>" (lvl''); iDestruct 1 as (lvl''' γ' Φ') "[#Hk' %Hsub']".
+  by iPoseProof (keyT_agree with "Hk Hk'") as "(<-&<-&_)".
 - case: lvl.
     iIntros "#Ht"; iExists Pub; iSplit=> //.
     by iIntros "!>" (lvl) "_".
-  iDestruct 1 as (lvl_enc lvl_dec Φ) "[#Hk #Ht]".
+  iDestruct 1 as (lvl_enc lvl_dec γ Φ) "[#Hk #Ht]".
   iDestruct "Ht" as "[[#Ht type]|[-> type]]"; last first.
-    iExists Pub; iSplit=> /=; first by iExists _, _, _; iSplit; eauto.
+    iExists Pub; iSplit=> /=; first by iExists _, _, _, _; iSplit; eauto.
     by iIntros "!>" (lvl) "_".
   iDestruct (IH with "type") as (lvl) "[type' #min']".
   case: lvl.
     iExists Pub; iSplit=> /=.
-      iExists _, _, _; iSplit=> //.
+      iExists _, _, _, _; iSplit=> //.
       by iLeft; iSplit=> //; case: lvl_dec.
     by iIntros "!>" (lvl) "_".
   case: lvl_dec.
     iExists Sec; iSplit=> /=.
-      iExists _, _, _; iSplit=> //.
+      iExists _, _, _, _; iSplit=> //.
       by iLeft; iSplit=> //; case: lvl_dec.
-    iIntros "!>" (lvl); iDestruct 1 as (lvl_enc' lvl_dec' Φ') "[#Hk' #type'']".
-    iDestruct (key_info_agree with "Hk Hk'") as "(_&<-&<-&_)".
+    iIntros "!>" (lvl).
+    iDestruct 1 as (lvl_enc' lvl_dec' γ' Φ') "[#Hk' #type'']".
+    iDestruct (key_info_agree with "Hk Hk'") as "(_&<-&<-&<-&_)".
     iDestruct "type''" as "[[_ type'']|[_ type'']]";
     iPoseProof ("min'" with "type''") as "?"=> //.
     by case: lvl.
   iExists Pub; iSplit=> /=.
-    iExists _, _, _; iSplit=> //.
+    iExists _, _, _, _; iSplit=> //.
     by iLeft; iSplit.
   by iIntros "!>" (lvl) "_".
 Qed.
@@ -457,14 +488,11 @@ Lemma res_alloc E r l :
   resT r l.
 Proof.
 iIntros (Hsub) "Hmeta".
-iMod (own_alloc (to_agree r)) as (γ) "#Hown" => //.
-iMod (meta_set E l γ with "Hmeta") as "Hmeta"=> //.
-by iModIntro; iExists γ; iSplit.
+iMod (meta_set E l r with "Hmeta") as "Hmeta"=> //.
 Qed.
 
 End Resources.
 
-Arguments RNonce {_} _.
-Arguments nonceT {_ _ _} _ _.
-Arguments skeyT {_ _ _} _ _ _.
-Arguments akeyT {_ _ _} _ _ _ _.
+Arguments nonceT {_ _} _ _.
+Arguments skeyT {_ _ _} _ _ _ _.
+Arguments akeyT {_ _ _} _ _ _ _ _.
